src/arch/x64/X64.Memory_i_s.fst
@@ -1,0 +1,432 @@
+module X64.Memory_i_s
+
+
+module HS = FStar.HyperStack
+module B = FStar.Buffer
+module M = FStar.Modifies
+module S = X64.Bytes_Semantics_s
+module H = FStar.Heap
+
+let heap = H.heap
+let mem = HS.mem
+
+let op_String_Access = Map.sel
+let op_String_Assignment = Map.upd
+
+let coerce (#a:Type0) (b:Type0{a == b}) (x:a) : b = x
+
+// TODO: Handle UInt128
+
+let tuint8 = UInt8.t
+let tuint16 = UInt16.t
+let tuint32 = UInt32.t
+let tuint64 = UInt64.t
+// let tuint128 = magic()
+
+let m_of_typ (t:typ) : Type0 =
+  match t with
+  | TBase TUInt8 -> tuint8
+  | TBase TUInt16 -> tuint16
+  | TBase TUInt32 -> tuint32
+  | TBase TUInt64 -> tuint64
+  | TBase TUInt128 -> admit () // M.tuint128
+
+let v_of_typ (t:typ) (v:type_of_typ t) :  (m_of_typ t) =
+  match t with
+  | TBase TUInt8 -> coerce ((m_of_typ t)) (UInt8.uint_to_t v)
+  | TBase TUInt16 -> coerce ((m_of_typ t)) (UInt16.uint_to_t v)
+  | TBase TUInt32 -> coerce ((m_of_typ t)) (UInt32.uint_to_t v)
+  | TBase TUInt64 -> coerce ((m_of_typ t)) (UInt64.uint_to_t v)
+  | TBase TUInt128 -> magic() //coerce (M.type_of_typ (m_of_typ t)) (UInt128.uint_to_t v)
+
+let v_to_typ (t:typ) (v:(m_of_typ t)) : type_of_typ t =
+  match t with
+  | TBase TUInt8 -> UInt8.v (coerce UInt8.t v)
+  | TBase TUInt16 -> UInt16.v (coerce UInt16.t v)
+  | TBase TUInt32 -> UInt32.v (coerce UInt32.t v)
+  | TBase TUInt64 -> UInt64.v (coerce UInt64.t v)
+  | TBase TUInt128 -> magic()
+  
+let lemma_v_to_of_typ (t:typ) (v:type_of_typ t) : Lemma
+  (ensures v_to_typ t (v_of_typ t v) == v)
+  [SMTPat (v_to_typ t (v_of_typ t v))]
+  =
+  match t with
+  | TBase TUInt8 -> assert (UInt8.v (UInt8.uint_to_t v) == v)
+  | TBase TUInt16 -> assert (UInt16.v (UInt16.uint_to_t v) == v)
+  | TBase TUInt32 -> assert (UInt32.v (UInt32.uint_to_t v) == v)
+  | TBase TUInt64 -> assert (UInt64.v (UInt64.uint_to_t v) == v)
+  | TBase TUInt128 -> admit()
+
+let buffer t = B.buffer (m_of_typ t)
+
+let buffer_as_seq #t h b =
+  let s = B.as_seq h b in
+  let len = Seq.length s in
+  let contents (i:nat{i < len}) : type_of_typ t = v_to_typ t (Seq.index s i) in
+  Seq.init len contents
+
+let buffer_readable #t h b = B.live h b
+let buffer_length #t b = B.length b
+let loc = M.loc
+let loc_none = M.loc_none
+let loc_union = M.loc_union
+let loc_buffer #t b = M.loc_buffer b
+let loc_disjoint = M.loc_disjoint
+let loc_includes = M.loc_includes
+let modifies = M.modifies
+
+let valid_state s = 
+  // Shouldn't be needed but logic annotation issue without it
+  let _ = () in
+  I.list_disjoint_or_eq #UInt64.t s.ptrs /\
+  I.list_live s.mem s.ptrs /\
+  s.state.S.mem == I.down_mem64 s.mem s.addrs s.ptrs
+
+let loc_readable h s = unit // admit()
+let loc_readable_none = admit()
+let loc_readable_union = admit()
+let loc_readable_buffer #t h b = admit()
+
+let modifies_goal_directed s h1 h2 = modifies s h1 h2
+let lemma_modifies_goal_directed s h1 h2 = ()
+
+let buffer_length_buffer_as_seq #t h b = ()
+
+val modifies_loc_readable (#t:typ) (b:buffer t) (p:loc) (h h':mem) : Lemma
+  (requires
+    loc_readable h' p /\
+    buffer_readable h b /\
+    modifies p h h'
+  )
+  (ensures
+    buffer_readable h' b
+  )
+
+let modifies_loc_readable #t b p h h' =
+  // TODO
+  admit ()
+
+let modifies_buffer_elim #t1 b p h h' =
+  if buffer_length b > 0 then
+  (
+    M.modifies_buffer_elim b p h h';
+    assert (Seq.equal (buffer_as_seq h b) (buffer_as_seq h' b));
+    ()
+  )
+  else
+  (
+    modifies_loc_readable b p h h';
+    assert (Seq.equal (buffer_as_seq h b) (buffer_as_seq h' b));
+    ()
+  )
+
+let loc_disjoint_none_r s = M.loc_disjoint_none_r s
+let loc_disjoint_union_r s s1 s2 = M.loc_disjoint_union_r s s1 s2
+let loc_includes_refl s = M.loc_includes_refl s
+let loc_includes_trans s1 s2 s3 = M.loc_includes_trans s1 s2 s3
+let loc_includes_union_r s s1 s2 = M.loc_includes_union_r s s1 s2
+let loc_includes_union_l s1 s2 s = M.loc_includes_union_l s1 s2 s
+let loc_includes_union_l_buffer #t s1 s2 b = M.loc_includes_union_l s1 s2 (loc_buffer b)
+let loc_includes_none s = M.loc_includes_none s
+let modifies_refl s h = M.modifies_refl s h
+let modifies_goal_directed_refl s h = M.modifies_refl s h
+let modifies_loc_includes s1 h h' s2 = M.modifies_loc_includes s1 h h' s2
+let modifies_trans s12 h1 h2 s23 h3 = M.modifies_trans s12 h1 h2 s23 h3
+
+let modifies_goal_directed_trans s12 h1 h2 s13 h3 =
+  modifies_trans s12 h1 h2 s13 h3;
+  modifies_loc_includes s13 h1 h3 (loc_union s12 s13);
+  ()
+
+let modifies_goal_directed_trans2 s12 h1 h2 s13 h3 = modifies_goal_directed_trans s12 h1 h2 s13 h3
+
+let default_of_typ (t:typ) : type_of_typ t =
+  match t with
+  | TBase TUInt8 -> 0
+  | TBase TUInt16 -> 0
+  | TBase TUInt32 -> 0
+  | TBase TUInt64 -> 0
+  | TBase TUInt128 -> Words_s.Mkfour #nat32 0 0 0 0
+
+let buffer_read #t b i h =
+  if i < 0 || i >= buffer_length b then default_of_typ t else
+  Seq.index (buffer_as_seq h b) i
+
+// Proven but private in FStar.Buffer
+assume private val lemma_aux: (#t:typ) -> b:buffer t -> n:nat{n < B.length b} -> z:m_of_typ t
+  -> h0:HS.mem -> Lemma
+  (requires True)
+  (ensures (B.live h0 b) ==> (B.live h0 b
+/\ B.modifies_1 b h0 (HS.upd h0 (B.content b) (Seq.upd (B.sel h0 b) (B.idx b + n) z)) ))
+
+let buffer_write #t b i v h =
+ if i < 0 || i >= buffer_length b then h else
+ begin
+ let vu = v_of_typ t v in
+ let s0 = B.sel h b in
+ let s = Seq.upd s0 (B.idx b + i) vu in
+ let h' = HS.upd h (B.content b) s in
+ lemma_aux b i vu h;
+ assert (Seq.equal (buffer_as_seq h' b) (Seq.upd (buffer_as_seq h b) i v));
+ h'
+ end
+
+let buffer_addr #t b s =
+  let addrs = s.addrs in
+  addrs.[(B.as_addr b, B.idx b, B.length b)]
+
+val addr_in_ptr: (addr:int) -> (ptr:buffer64) -> (s:state) ->
+  GTot (b:bool{ not b <==> (forall i. 0 <= i /\ i < B.length ptr ==> 
+    addr <> (buffer_addr ptr s) + 8 `op_Multiply` i)})
+  
+// Checks if address addr corresponds to one of the elements of buffer ptr
+let addr_in_ptr (addr:int) (ptr:buffer64) (s:state) =
+  let n = B.length ptr in
+  let base = buffer_addr ptr s in
+  let rec aux (i:nat) : Tot (b:bool{not b <==> (forall j. i <= j /\ j < n ==> 
+    addr <> base + 8 `op_Multiply` j)}) 
+    (decreases %[n-i]) =
+    if i >= n then false
+    else if addr = base + 8 `op_Multiply` i then true
+    else aux (i+1)
+  in aux 0
+
+let rec get_addr_in_ptr (n base addr:nat) (i:nat{exists j. i <= j /\ j < n /\ base + 8 `op_Multiply` j == addr}) : 
+    GTot (j:nat{base + 8 `op_Multiply` j == addr})
+    (decreases %[n-i]) =
+    if base + 8 `op_Multiply` i = addr then i
+    else if i >= n then i
+    else get_addr_in_ptr n base addr (i+1)
+
+
+let rec valid_mem_aux addr ps (s:state) : GTot (b:bool{
+  (not b) <==> (forall (x:buffer64). (List.memP x ps ==> not (addr_in_ptr addr x s) ))}) 
+  = match ps with
+    | [] -> false
+    | a::q -> if (addr_in_ptr addr a s) then true else valid_mem_aux addr q s
+
+let valid_mem64 ptr s = valid_mem_aux ptr s.ptrs s
+
+// TODO: Probably a similar approach baser on buffer_read?
+let load_mem64 ptr s = S.get_heap_val64 ptr s.state.S.mem
+
+let rec store_mem_aux addr ps (v:nat64) (s:state) (h0:HS.mem{I.list_live h0 ps}) : 
+  GTot (h1:HS.mem{forall (b:buffer64). B.live h0 b <==> B.live h1 b }) =
+  match ps with
+  | [] -> h0
+  | a::q ->
+    let base = buffer_addr a s in
+    let n = B.length a in
+    if addr_in_ptr addr a s then
+    begin
+      buffer_write a (get_addr_in_ptr n base addr 0) v h0
+    end
+    else store_mem_aux addr q v s h0
+
+#set-options "--z3rlimit 40"
+
+let rec written_buffer_down_aux1 (b:buffer64) (i:nat{i < B.length b}) (v:nat64)
+      (ps:list buffer64{I.list_disjoint_or_eq ps /\ List.memP b ps})
+      (h0:HS.mem{I.list_live h0 ps}) (s:state)
+      (base:nat{base == buffer_addr b s})
+      (k:nat) (h1:HS.mem{h1 == buffer_write b i v h0}) 
+      (mem1:S.heap{I.correct_down64 h0 s.addrs ps mem1}) 
+      (mem2:S.heap{
+      (I.correct_down64 h1 s.addrs ps mem2) /\
+      (forall j. base <= j /\ j < base + k `op_Multiply` 8 ==> mem1.[j] == mem2.[j])}) : 
+      Lemma (requires True)
+      (ensures (forall j. j >= base /\ j < base + 8 `op_Multiply` i ==> mem1.[j] == mem2.[j]))
+      (decreases %[i-k]) =
+    if k >= i then ()
+    else begin
+      assert (Seq.index (B.as_seq h0 b) k == Seq.index (B.as_seq h1 b) k);
+      Bytes_Semantics_i.same_mem_get_heap_val (base + 8 `op_Multiply` k) mem1 mem2;
+      written_buffer_down_aux1 b i v ps h0 s base (k+1) h1 mem1 mem2
+    end
+
+let rec written_buffer_down_aux2 (b:buffer64) (i:nat{i < B.length b}) (v:nat64)
+      (ps:list buffer64{I.list_disjoint_or_eq ps /\ List.memP b ps})
+      (h0:HS.mem{I.list_live h0 ps}) (s:state)
+      (base:nat{base == buffer_addr b s})
+      (n:nat{n == B.length b})
+      (k:nat{k > i}) (h1:HS.mem{h1 == buffer_write b i v h0}) 
+      (mem1:S.heap{I.correct_down64 h0 s.addrs ps mem1}) 
+      (mem2:S.heap{
+      (I.correct_down64 h1 s.addrs ps mem2) /\
+      (forall j. base + 8 `op_Multiply` (i+1) <= j /\ j < base + k `op_Multiply` 8 ==>
+      mem1.[j] == mem2.[j])}) :
+      Lemma 
+      (requires True)
+      (ensures (forall j. j >= base + 8 `op_Multiply` (i+1) /\ j < base + 8 `op_Multiply` n ==> 
+	mem1.[j] == mem2.[j]))
+      (decreases %[n-k]) =
+    if k >= n then ()
+    else begin
+      assert (Seq.index (B.as_seq h0 b) k == Seq.index (B.as_seq h1 b) k);
+      Bytes_Semantics_i.same_mem_get_heap_val (base + 8 `op_Multiply` k) mem1 mem2;
+      written_buffer_down_aux2 b i v ps h0 s base n (k+1) h1 mem1 mem2
+    end
+    
+let written_buffer_down (b:buffer64) (i:nat{i < B.length b}) (v:nat64)
+  (ps: list buffer64{I.list_disjoint_or_eq ps /\ List.memP b ps}) (h0:HS.mem{I.list_live h0 ps}) (s:state) :
+  Lemma (
+    let mem1 = I.down_mem64 h0 s.addrs ps in
+    let h1 = buffer_write b i v h0 in
+    let mem2 = I.down_mem64 h1 s.addrs ps in
+    let base = buffer_addr b s in
+    let n = B.length b in
+    forall j. (base <= j /\ j < base + 8 `op_Multiply` i) \/ 
+	 (base + 8 `op_Multiply` (i+1) <= j /\ j < base + 8 `op_Multiply` n) ==>
+	 mem1.[j] == mem2.[j]) = 
+    let mem1 = I.down_mem64 h0 s.addrs ps in
+    let h1 = buffer_write b i v h0 in
+    let mem2 = I.down_mem64 h1 s.addrs ps in	 
+    let base = buffer_addr b s in
+    let n = B.length b in
+    written_buffer_down_aux1 b i v ps h0 s base 0 h1 mem1 mem2;
+    written_buffer_down_aux2 b i v ps h0 s base n (i+1) h1 mem1 mem2
+
+let same_mem_get_heap_val_buf (base n:int) (mem1 mem2:S.heap) : Lemma
+  (requires (forall i. 0 <= i /\ i < n ==> 
+    S.get_heap_val64 (base + 8 `op_Multiply` i) mem1 == S.get_heap_val64 (base + 8 `op_Multiply` i) mem2))
+  (ensures (forall i. i >= base /\ i < base + n `op_Multiply` 8 ==> mem1.[i] == mem2.[i])) =
+  let rec aux (k:nat) : Lemma
+  (requires (forall i. i >= base /\ i < base + k `op_Multiply` 8 ==> mem1.[i] == mem2.[i]) /\
+   (forall i. 0 <= i /\ i < n ==> 
+    S.get_heap_val64 (base + 8 `op_Multiply` i) mem1 == S.get_heap_val64 (base + 8 `op_Multiply` i) mem2) 
+  )
+  (ensures (forall i. i >= base /\ i < base + n `op_Multiply` 8 ==> mem1.[i] == mem2.[i]))
+  (decreases %[n-k]) =
+  if k >= n then ()
+  else begin
+    Bytes_Semantics_i.same_mem_get_heap_val (base + k `op_Multiply` 8) mem1 mem2;
+    aux (k+1)
+  end
+  in aux 0
+
+let rec unwritten_buffer_down_aux (b:buffer64) (i:nat{i < B.length b}) (v:nat64)
+  (ps: list buffer64{I.list_disjoint_or_eq ps /\ List.memP b ps})
+  (h0:HS.mem{I.list_live h0 ps}) 
+  (s:state) (a:buffer64{a =!= b /\ List.memP a ps})  : 
+  Lemma (let base = buffer_addr a s in
+    let mem1 = I.down_mem64 h0 s.addrs ps in
+    let h1 = buffer_write b i v h0 in
+    let mem2 = I.down_mem64 h1 s.addrs ps in
+    forall j. j >= base /\ j < base + (B.length a) `op_Multiply` 8 ==> mem1.[j] == mem2.[j]) =
+    let mem1 = I.down_mem64 h0 s.addrs ps in
+    let h1 = buffer_write b i v h0 in
+    let mem2 = I.down_mem64 h1 s.addrs ps in
+    let base = buffer_addr a s in    
+    let s0 = B.as_seq h0 a in
+    assert (I.disjoint_or_eq a b);
+    // We need this to help z3
+    assert (forall j. 0 <= j /\ j < B.length a ==> UInt64.v (Seq.index s0 j) == S.get_heap_val64 (base + (j `op_Multiply` 8)) mem1 );
+    same_mem_get_heap_val_buf base (B.length a) mem1 mem2
+
+let unwritten_buffer_down (b:buffer64) (i:nat{i < B.length b}) (v:nat64)
+  (ps: list buffer64{I.list_disjoint_or_eq ps /\ List.memP b ps}) (h0:HS.mem{I.list_live h0 ps}) (s:state) : Lemma (
+    let mem1 = I.down_mem64 h0 s.addrs ps in
+    let h1 = buffer_write b i v h0 in
+    let mem2 = I.down_mem64 h1 s.addrs ps in
+    forall  (a:buffer64{List.memP a ps /\ a =!= b}) j.
+    let base = buffer_addr a s in j >= base /\ j < base + B.length a `op_Multiply` 8 ==> mem1.[j] == mem2.[j]) =
+    let mem1 = I.down_mem64 h0 s.addrs ps in
+    let h1 = buffer_write b i v h0 in
+    let mem2 = I.down_mem64 h1 s.addrs ps in   
+    let fintro (a:buffer64{List.memP a ps /\ a =!= b}) 
+      : Lemma 
+      (forall j. let base = buffer_addr a s in 
+      j >= base /\ j < base + (B.length a) `op_Multiply` 8 ==> 
+	mem1.[j] == mem2.[j]) =
+      let base = buffer_addr a s in
+      unwritten_buffer_down_aux b i v ps h0 s a
+    in
+    Classical.forall_intro fintro
+
+let store_buffer_down_mem (b:buffer64) (i:nat{i < B.length b}) (v:nat64)
+  (ps: list buffer64{I.list_disjoint_or_eq ps /\ List.memP b ps}) (h0:HS.mem{I.list_live h0 ps}) (s:state) :
+  Lemma (
+    let mem1 = I.down_mem64 h0 s.addrs ps in
+    let h1 = buffer_write b i v h0 in
+    let mem2 = I.down_mem64 h1 s.addrs ps in
+    let base = buffer_addr b s in
+    forall j. j < base + 8 `op_Multiply` i \/ j >= base + 8 `op_Multiply` (i+1) ==>
+      mem1.[j] == mem2.[j]) =
+    let mem1 = I.down_mem64 h0 s.addrs ps in
+    let h1 = buffer_write b i v h0 in
+    let mem2 = I.down_mem64 h1 s.addrs ps in
+    let base = buffer_addr b s in
+    let n = B.length b in
+    I.same_unspecified_down h0 h1 s.addrs ps;
+    unwritten_buffer_down b i v ps h0 s;
+    assert (forall j. (exists (a:buffer64{List.memP a ps /\ a =!= b}) . let base = buffer_addr a s in
+      j >= base /\ j < base + B.length a `op_Multiply` 8) ==> mem1.[j] == mem2.[j]);
+
+    written_buffer_down b i v ps h0 s;
+    ()
+
+let rec get_addr_ptr (ptr:int) (s:state) (ps:list buffer64{valid_mem_aux ptr ps s}) : 
+  GTot (b:buffer64{List.memP b ps /\ addr_in_ptr ptr b s}) =
+  match ps with
+  // The list cannot be empty because of the mem predicate
+  | a::q -> if addr_in_ptr ptr a s then a else get_addr_ptr ptr s q
+
+let store_buffer_aux_down_mem (ptr:int) (v:nat64) (s:state{valid_mem64 ptr s}) : Lemma (
+  let mem1 = I.down_mem64 s.mem s.addrs s.ptrs in
+  let h1 = store_mem_aux ptr s.ptrs v s s.mem in
+  let mem2 = I.down_mem64 h1 s.addrs s.ptrs in
+  forall j. j < ptr \/ j >= ptr + 8 ==> mem1.[j] == mem2.[j]) =
+  let h1 = store_mem_aux ptr s.ptrs v s s.mem in
+  let b = get_addr_ptr ptr s s.ptrs in
+  let i = get_addr_in_ptr (B.length b) (buffer_addr b s) ptr 0 in
+  let rec aux (ps:list buffer64{I.list_disjoint_or_eq ps /\ valid_mem_aux ptr ps s}) (h:HS.mem{I.list_live h ps}) :
+  Lemma (let b = get_addr_ptr ptr s ps in
+    let i = get_addr_in_ptr (B.length b) (buffer_addr b s) ptr 0 in
+    store_mem_aux ptr ps v s h == buffer_write b i v h) =
+    match ps with
+    | [] -> ()
+    | a::q ->
+      if addr_in_ptr ptr a s then () else aux q h    
+  in aux s.ptrs s.mem;
+  store_buffer_down_mem b i v s.ptrs s.mem s
+
+let store_buffer_aux_down_mem2 (ptr:int) (v:nat64) (s:state{valid_mem64 ptr s}) : Lemma (
+  let h1 = store_mem_aux ptr s.ptrs v s s.mem in
+  let mem2 = I.down_mem64 h1 s.addrs s.ptrs in
+  S.get_heap_val64 ptr mem2 == v) =
+  let b = get_addr_ptr ptr s s.ptrs in
+  let i = get_addr_in_ptr (B.length b) (buffer_addr b s) ptr 0 in
+  let h1 = store_mem_aux ptr s.ptrs v s s.mem in
+  let mem2 = I.down_mem64 h1 s.addrs s.ptrs in
+  let rec aux (ps:list buffer64{I.list_disjoint_or_eq ps /\ valid_mem_aux ptr ps s}) (h:HS.mem{I.list_live h ps}) :
+  Lemma (let b = get_addr_ptr ptr s ps in
+    let i = get_addr_in_ptr (B.length b) (buffer_addr b s) ptr 0 in
+    store_mem_aux ptr ps v s h == buffer_write b i v h) =
+    match ps with
+    | [] -> ()
+    | a::q ->
+      if addr_in_ptr ptr a s then () else aux q h    
+  in aux s.ptrs s.mem;
+  assert (UInt64.v (Seq.index (B.as_seq h1 b) i) == v);
+  ()
+
+#set-options "--z3rlimit 60"
+
+let store_mem64 i v s =
+  if not (valid_mem64 i s) then s
+  else
+  let s' = S.update_mem i v s.state in
+  let h1 = store_mem_aux i s.ptrs v s s.mem in
+  let s' = {s with state = s'; mem = h1} in
+  Bytes_Semantics_i.frame_update_heap i v s.state.S.mem;
+  store_buffer_aux_down_mem i v s;
+  store_buffer_aux_down_mem2 i v s;
+  let mem1 = s'.state.S.mem in
+  let mem2 = I.down_mem64 s'.mem s.addrs s.ptrs in
+  Bytes_Semantics_i.same_mem_get_heap_val i mem1 mem2;
+  Bytes_Semantics_i.correct_update_get i v s.state.S.mem;
+  assert (forall j. mem1.[j] == mem2.[j]);
+  assert (Map.equal mem1 mem2);
+  s'
+
